WIP

theories/Interp/State.v
@@ -3,35 +3,42 @@ From ExtLib Require Import
      Structures.Monad.
 
 From ITree Require Import
-	   Basics.CategoryOps.
-
-From CTree Require Import
-     CTree Interp.Interp.
+     Subevent
+     CategoryOps
+     Indexed.Sum.
 
 Import ITree.Basics.Basics.Monads.
+
+From CTree Require Import
+     CTrees
+     CTreesTheory
+     Utils
+     Interp
+     Equ.
+
 Import MonadNotation.
 Open Scope monad_scope.
+
+Set Implicit Arguments.
+Set Strict Implicit.
 
 (* Stateful handlers [E ~> stateT S (itree F)] and morphisms
    [E ~> state S] define stateful itree morphisms
    [itree E ~> stateT S (itree F)]. *)
 
-#[global] Instance MonadChoice_stateT {M S} {MM : Monad M} {AM : MonadChoice M}: MonadChoice (stateT S M) :=
-  fun b n s =>
-    f <- choice b n;;
-    ret (s, f).
-
-Definition interp_state {E M S}
-           {FM : Functor M} {MM : Monad M}
-           {IM : MonadIter M}{MC: MonadChoice M} (h : E ~> stateT S M) :
-  ctree E ~> stateT S M := interp h.
-
-Arguments interp_state {E M S FM MM IM MC} h [T].
-
 Section State.
 
   Variable (S : Type).
 
+  #[global] Instance MonadChoice_stateT {M} {MM : Monad M} {AM : MonadChoice M}: MonadChoice (stateT S M) :=
+  fun b n s =>
+    f <- choice b n;;
+    ret (s, f).
+
+  Definition interp_state {E M}
+           {FM : Functor M} {MM : Monad M}
+           {IM : MonadIter M}{MC: MonadChoice M} (h : E ~> stateT S M) :
+    ctree E ~> stateT S M := interp h.
   Variant stateE : Type -> Type :=
   | Get : stateE S
   | Put : S -> stateE unit.
@@ -52,9 +59,275 @@ Section State.
   Definition run_state {E}
     : ctree (stateE +' E) ~> stateT S (ctree E)
     := interp_state (case_ h_state pure_state).
+  
+  (** Facts about state (equational theory) *)
+  Definition _interp_state {E F R}
+           (f : E ~> stateT S (ctree F)) (ot : ctreeF E R _)
+  : stateT S (ctree F) R := fun s =>
+  match ot with
+  | RetF r => Ret (s, r)
+  | ChoiceF b n' k =>
+      Choice b n' (fun i => interp_state f (k i) s)
+  | VisF e k => f _ e s >>= (fun sx => TauI (interp_state f (k (snd sx)) (fst sx)))
+  end.
+
+                          Lemma unfold_interp_state {E F R} (h : E ~> Monads.stateT S (ctree F))
+        (t : ctree E R) s :
+    interp_state h t s ≅ _interp_state h (observe t) s.
+  Proof.
+    unfold interp_state, interp, Basics.iter, MonadIter_stateT0, Basics.iter, MonadIter_ctree; cbn.
+    rewrite unfold_iter; cbn.
+    destruct observe; cbn.
+    - rewrite 2 bind_ret_l. reflexivity.
+    - rewrite bind_map, bind_bind; cbn. setoid_rewrite bind_ret_l.
+      cbn. apply eqit_bind; reflexivity.
+  Qed.
 
 End State.
 
 Arguments get {S E _}.
 Arguments put {S E _}.
 Arguments run_state {S E} [_] _ _.
+Arguments interp_state {S E M FM MM IM MC} h [T].
+
+
+#[global]
+Instance eq_itree_interp_state {E F S R} (h : E ~> Monads.stateT S (itree F)) :
+q  Proper (eq_itree eq ==> eq ==> eq_itree eq)
+         (@interp_state _ _ _ _ _ _ h R).
+Proof.
+  revert_until R.
+  ginit. pcofix CIH. intros h x y H0 x2 _ [].
+  rewrite !unfold_interp_state.
+  punfold H0; repeat red in H0.
+  destruct H0; subst; pclearbot; try discriminate; cbn.
+  - gstep; constructor; auto.
+  - gstep; constructor; auto with paco.
+  - guclo eqit_clo_bind. econstructor.
+    + reflexivity.
+    + intros [] _ []. gstep; constructor; auto with paco itree.
+Qed.
+
+Lemma interp_state_ret {E F : Type -> Type} {R S : Type}
+      (f : forall T, E T -> S -> itree F (S * T)%type)
+      (s : S) (r : R) :
+  (interp_state f (Ret r) s) ≅ (Ret (s, r)).
+Proof.
+  rewrite itree_eta. reflexivity.
+Qed.
+
+Lemma interp_state_vis {E F : Type -> Type} {S T U : Type}
+      (e : E T) (k : T -> itree E U) (h : E ~> Monads.stateT S (itree F)) (s : S)
+  : interp_state h (Vis e k) s
+  ≅ h T e s >>= fun sx => Tau (interp_state h (k (snd sx)) (fst sx)).
+Proof.
+  rewrite unfold_interp_state; reflexivity.
+Qed.
+
+Lemma interp_state_tau {E F : Type -> Type} S {T : Type}
+      (t : itree E T) (h : E ~> Monads.stateT S (itree F)) (s : S)
+  : interp_state h (Tau t) s ≅ Tau (interp_state h t s).
+Proof.
+  rewrite unfold_interp_state; reflexivity.
+Qed.
+
+Lemma interp_state_trigger_eqit {E F : Type -> Type} {R S : Type}
+      (e : E R) (f : E ~> Monads.stateT S (itree F)) (s : S)
+  : (interp_state f (ITree.trigger e) s) ≅ (f _ e s >>= fun x => Tau (Ret x)).
+Proof.
+  unfold ITree.trigger. rewrite interp_state_vis.
+  eapply eqit_bind; try reflexivity.
+  intros []. rewrite interp_state_ret. reflexivity.
+Qed.
+
+Lemma interp_state_trigger {E F : Type -> Type} {R S : Type}
+      (e : E R) (f : E ~> Monads.stateT S (itree F)) (s : S)
+  : interp_state f (ITree.trigger e) s ≈ f _ e s.
+Proof.
+  unfold ITree.trigger. rewrite interp_state_vis.
+  match goal with
+    |- ?y ≈ ?x => remember y; rewrite <- (bind_ret_r x); subst
+  end.
+  eapply eqit_bind; try reflexivity.
+  intros []; rewrite interp_state_ret,tau_eutt.
+  reflexivity.
+Qed.
+
+Lemma interp_state_bind {E F : Type -> Type} {A B S : Type}
+      (f : forall T, E T -> S -> itree F (S * T)%type)
+      (t : itree E A) (k : A -> itree E B)
+      (s : S) :
+  (interp_state f (t >>= k) s)
+    ≅
+  (interp_state f t s >>= fun st => interp_state f (k (snd st)) (fst st)).
+Proof.
+  revert t k s.
+  ginit. pcofix CIH.
+  intros t k s.
+  rewrite unfold_bind.
+  rewrite (unfold_interp_state f t).
+  destruct (observe t).
+  - cbn. rewrite !bind_ret_l. cbn.
+    apply reflexivity.
+  - cbn. rewrite !bind_tau, interp_state_tau.
+    gstep. econstructor. gbase. apply CIH.
+  - cbn. rewrite interp_state_vis, bind_bind.
+    guclo eqit_clo_bind. econstructor.
+    + reflexivity.
+    + intros u2 ? [].
+      rewrite bind_tau.
+      gstep; constructor.
+      ITree.fold_subst.
+      auto with paco.
+Qed.
+
+#[global]
+Instance eutt_interp_state {E F: Type -> Type} {S : Type}
+         (h : E ~> Monads.stateT S (itree F)) R RR :
+  Proper (eutt RR ==> eq ==> eutt (prod_rel eq RR)) (@interp_state E (itree F) S _ _ _ h R).
+Proof.
+  repeat intro. subst. revert_until RR.
+  einit. ecofix CIH. intros.
+
+  rewrite !unfold_interp_state. punfold H0. red in H0.
+  induction H0; intros; subst; simpl; pclearbot.
+  - eret.
+  - etau.
+  - ebind. econstructor; [reflexivity|].
+    intros; subst.
+    etau. ebase.
+  - rewrite tau_euttge, unfold_interp_state; eauto.
+  - rewrite tau_euttge, unfold_interp_state; eauto.
+Qed.
+
+#[global]
+Instance eutt_interp_state_eq {E F: Type -> Type} {S : Type}
+         (h : E ~> Monads.stateT S (itree F)) R :
+  Proper (eutt eq ==> eq ==> eutt eq) (@interp_state E (itree F) S _ _ _ h R).
+Proof.
+  repeat intro. subst. revert_until R.
+  einit. ecofix CIH. intros.
+
+  rewrite !unfold_interp_state. punfold H0. red in H0.
+  induction H0; intros; subst; simpl; pclearbot.
+  - eret.
+  - etau.
+  - ebind. econstructor; [reflexivity|].
+    intros; subst.
+    etau. ebase.
+  - rewrite tau_euttge, unfold_interp_state; eauto.
+  - rewrite tau_euttge, unfold_interp_state; eauto.
+Qed.
+
+
+Lemma eutt_interp_state_aloop {E F S I I' A A'}
+      (RA : A -> A' -> Prop) (RI : I -> I' -> Prop)
+      (RS : S -> S -> Prop)
+      (h : E ~> Monads.stateT S (itree F))
+      (t1 : I -> itree E (I + A))
+      (t2 : I' -> itree E (I' + A')):
+  (forall i i' s1 s2, RS s1 s2 -> RI i i' ->
+     eutt (prod_rel RS (sum_rel RI RA))
+                     (interp_state h (t1 i) s1)
+                     (interp_state h (t2 i') s2)) ->
+  (forall i i' s1 s2, RS s1 s2 -> RI i i' ->
+     eutt (fun a b => RS (fst a) (fst b) /\ RA (snd a) (snd b))
+          (interp_state h (ITree.iter t1 i) s1)
+          (interp_state h (ITree.iter t2 i') s2)).
+Proof.
+  intro Ht.
+  einit. ecofix CIH. intros.
+  rewrite 2 unfold_iter.
+  rewrite 2 interp_state_bind.
+  ebind; econstructor.
+  - eapply Ht; auto.
+  - intros [s1' i1'] [s2' i2'] [? []]; cbn.
+    + rewrite 2 interp_state_tau. auto with paco.
+    + rewrite 2 interp_state_ret. auto with paco.
+Qed.
+
+Lemma eutt_interp_state_iter {E F S A A' B B'}
+      (RA : A -> A' -> Prop) (RB : B -> B' -> Prop)
+      (RS : S -> S -> Prop)
+      (h : E ~> Monads.stateT S (itree F))
+      (t1 : A -> itree E (A + B))
+      (t2 : A' -> itree E (A' + B')) :
+  (forall ca ca' s1 s2, RS s1 s2 ->
+                        RA ca ca' ->
+     eutt (prod_rel RS (sum_rel RA RB))
+          (interp_state h (t1 ca) s1)
+          (interp_state h (t2 ca') s2)) ->
+  (forall a a' s1 s2, RS s1 s2 -> RA a a' ->
+     eutt (fun a b => RS (fst a) (fst b) /\ RB (snd a) (snd b))
+          (interp_state h (iter (C := ktree _) t1 a) s1)
+          (interp_state h (iter (C := ktree _) t2 a') s2)).
+Proof.
+  apply eutt_interp_state_aloop.
+Qed.
+
+Lemma eutt_interp_state_loop {E F S A B C} (RS : S -> S -> Prop)
+      (h : E ~> Monads.stateT S (itree F))
+      (t1 t2 : C + A -> itree E (C + B)) :
+  (forall ca s1 s2, RS s1 s2 ->
+     eutt (fun a b => RS (fst a) (fst b) /\ snd a = snd b)
+          (interp_state h (t1 ca) s1)
+          (interp_state h (t2 ca) s2)) ->
+  (forall a s1 s2, RS s1 s2 ->
+     eutt (fun a b => RS (fst a) (fst b) /\ snd a = snd b)
+          (interp_state h (loop (C := ktree E) t1 a) s1)
+          (interp_state h (loop (C := ktree E) t2 a) s2)).
+Proof.
+  intros.
+  unfold loop, bimap, Bimap_Coproduct, case_, Case_Kleisli, Function.case_sum, id_, Id_Kleisli, cat, Cat_Kleisli, inr_, Inr_Kleisli, inl_, Inl_Kleisli, lift_ktree_; cbn.
+  rewrite 2 bind_ret_l.
+  eapply (eutt_interp_state_iter eq eq); auto; intros.
+  rewrite 2 interp_state_bind.
+  subst.
+  eapply eutt_clo_bind; eauto.
+  intros.
+  cbn in H2; destruct (snd u1); rewrite <- (proj2 H2).
+  - rewrite bind_ret_l, 2 interp_state_ret.
+    pstep.
+    constructor.
+    split; cbn; auto using (proj1 H2).
+  - rewrite bind_ret_l, 2 interp_state_ret. pstep. constructor.
+    split; cbn; auto using (proj1 H2).
+Qed.
+
+(* SAZ: These are probably too specialized. *)
+Definition state_eq {E S X}
+  : (stateT S (itree E) X) -> (stateT S (itree E) X) -> Prop :=
+  fun t1 t2 => forall s, eq_itree eq (t1 s) (t2 s).
+
+Lemma interp_state_iter {E F } S (f : E ~> stateT S (itree F)) {I A}
+      (t  : I -> itree E (I + A))
+      (t' : I -> stateT S (itree F) (I + A))
+      (EQ_t : forall i, state_eq (State.interp_state f (t i)) (t' i))
+  : forall i, state_eq (State.interp_state f (ITree.iter t i))
+                  (Basics.iter t' i).
+Proof.
+  unfold Basics.iter, MonadIter_stateT0, Basics.iter, MonadIter_itree in *; cbn.
+  ginit. pcofix CIH; intros i s.
+  rewrite 2 unfold_iter; cbn.
+  rewrite !bind_bind.
+  setoid_rewrite bind_ret_l.
+  rewrite interp_state_bind.
+  guclo eqit_clo_bind; econstructor; eauto.
+  - apply EQ_t.
+  - intros [s' []] _ []; cbn.
+    + rewrite interp_state_tau.
+      gstep; constructor.
+      auto with paco.
+    + rewrite interp_state_ret; apply reflexivity.
+Qed.
+
+Lemma interp_state_iter' {E F } S (f : E ~> stateT S (itree F)) {I A}
+      (t  : I -> itree E (I + A))
+  : forall i, state_eq (State.interp_state f (ITree.iter t i))
+                       (Basics.iter (fun i => State.interp_state f (t i)) i).
+Proof.
+  eapply interp_state_iter.
+  intros i.
+  red. reflexivity.
+Qed.
+
